Clean up a little; notation.

Trivalent.v
@@ -2,11 +2,13 @@
 Inductive T :=
 | true : T
 | false : T.
+Notation "⊤" := true.
+Notation "⊥" := false.
 
 Definition T_elim {a : Type} (p : T) (v1 v2 : a) : a :=
   match p with
-  | true => v1
-  | false => v2
+  | ⊤ => v1
+  | ⊥ => v2
   end.
 
 (* Convenient to have. *)
@@ -28,26 +30,28 @@ Inductive THash :=
 | trueHash : THash
 | falseHash : THash
 | hash : THash.
+Notation "T#" := THash.
+Notation "⊤#" := trueHash.
+Notation "⊥#" := falseHash.
+Notation "#" := hash.
 
-Definition THash_elim {a : Type} (p : THash) (v1 v2 v3 : a) : a :=
+Definition THash_elim {a : Type} (p : T#) (v1 v2 v3 : a) : a :=
   match p with
-  | trueHash => v1
-  | falseHash => v2
-  | hash => v3
+  | ⊤# => v1
+  | ⊥# => v2
+  | # => v3
   end.
 
 (* Convienent to have. *)
-Theorem THash_not_eq : ~ (trueHash = falseHash) /\
-                         ~ (hash = trueHash) /\
-                         ~ (hash = falseHash).
+Theorem THash_not_eq : ~ (⊤# = ⊥#) /\ ~ (# = ⊤#) /\ ~ (# = ⊥#).
 Proof.
   split.
   intro.
-  pose (eq_refl (THash_elim trueHash unit False unit)).
-  replace (THash_elim trueHash unit False unit =
-             THash_elim trueHash unit False unit) with
-    (THash_elim trueHash unit False unit =
-       THash_elim falseHash unit False unit)
+  pose (eq_refl (THash_elim ⊤# unit False unit)).
+  replace (THash_elim ⊤# unit False unit =
+             THash_elim ⊤# unit False unit) with
+    (THash_elim ⊤# unit False unit =
+       THash_elim ⊥# unit False unit)
     in e by now (rewrite H).
   pose tt.
   unfold THash_elim in e.
@@ -55,22 +59,22 @@ Proof.
   exact u.
   split.
   intro.
-  pose (eq_refl (THash_elim trueHash unit unit False)).
-  replace (THash_elim trueHash unit unit False =
-             THash_elim trueHash unit unit False) with
-    (THash_elim trueHash unit unit False =
-       THash_elim hash unit unit False)
+  pose (eq_refl (THash_elim ⊤# unit unit False)).
+  replace (THash_elim ⊤# unit unit False =
+             THash_elim ⊤# unit unit False) with
+    (THash_elim ⊤# unit unit False =
+       THash_elim # unit unit False)
     in e by now (rewrite H).
   pose tt.
   unfold THash_elim in e.
   rewrite e in u.
   exact u.
   intro.
-  pose (eq_refl (THash_elim falseHash unit unit False)).
-  replace (THash_elim falseHash unit unit False =
-             THash_elim falseHash unit unit False) with
-    (THash_elim falseHash unit unit False =
-       THash_elim hash unit unit False)
+  pose (eq_refl (THash_elim ⊥# unit unit False)).
+  replace (THash_elim ⊥# unit unit False =
+             THash_elim ⊥# unit unit False) with
+    (THash_elim ⊥# unit unit False =
+       THash_elim # unit unit False)
     in e by now (rewrite H).
   pose tt.
   unfold THash_elim in e.
@@ -79,102 +83,31 @@ Proof.
 Qed.
 
 (* The ``charitable'' trivalent existential quantifier, ∃#. *)
-Parameter existsHash : forall {a : Set}, (a -> THash) -> THash.
-Axiom existsHashDef1 : forall {a : Set} {k : a -> THash},
-    (exists (x : a), k x = trueHash) -> existsHash k = trueHash.
-Axiom existsHashDef1' : forall {a : Set} {k : a -> THash},
-    existsHash k = trueHash -> (exists (x : a), k x = trueHash).
-Axiom existsHashDef2 : forall {a : Set} {k : a -> THash},
-    ((exists (x : a), k x = falseHash) /\ ~ (exists (x : a), k x = trueHash)) ->
-    existsHash k = falseHash.
-Axiom existsHashDef2' : forall {a : Set} {k : a -> THash},
-    existsHash k = falseHash ->
-    (exists (x : a), k x = falseHash) /\ ~ (exists (x : a), k x = trueHash).
-Axiom existsHashDef3 : forall {a : Set} {k : a -> THash},
-    (forall (x : a), k x = hash) -> existsHash k = hash.
-Axiom existsHashDef3' : forall {a : Set} {k : a -> THash},
-    existsHash k = hash -> (forall (x : a), k x = hash).
+Parameter existsHash : forall {a : Set}, (a -> T#) -> T#.
+Notation "∃# P" := (existsHash P) (at level 200).
+Axiom existsHashDef1 :
+  forall {a : Set} {k : a -> T#}, (exists (x : a), k x = ⊤#) -> (∃# k) = ⊤#.
+Axiom existsHashDef1' :
+  forall {a : Set} {k : a -> T#}, (∃# k) = ⊤# -> (exists (x : a), k x = ⊤#).
+Axiom existsHashDef2 :
+  forall {a : Set} {k : a -> T#},
+    (exists (x : a), k x = ⊥#) /\ ~ (exists (x : a), k x = ⊤#) -> (∃# k) = ⊥#.
+Axiom existsHashDef2' :
+  forall {a : Set} {k : a -> T#},
+    (∃# k) = ⊥# -> (exists (x : a), k x = ⊥#) /\ ~ (exists (x : a), k x = ⊤#).
+Axiom existsHashDef3 :
+  forall {a : Set} {k : a -> T#}, (forall (x : a), k x = #) -> (∃# k) = #.
+Axiom existsHashDef3' :
+  forall {a : Set} {k : a -> T#}, (∃# k) = # -> (forall (x : a), k x = #).
 
-Lemma existsHash_comm : forall {a : Set} {b : Set} {k : a * b -> THash},
-    existsHash (fun x : a => existsHash (fun (y : b) => k (x, y))) =
-      existsHash (fun y : b => existsHash (fun (x : a) => k (x, y))).
-Proof.
-  intros.
-  case_eq (existsHash (fun x : a => existsHash (fun (y : b) => k (x, y)))).
-  intros.
-  pose (existsHashDef1' H).
-  elim e.
-  intros.
-  pose (existsHashDef1' H0).
-  elim e0.
-  intros.
-  pose (existsHashDef1 (ex_intro (fun (x1 : a) => k (x1, x0) = trueHash) x H1)).
-  pose (existsHashDef1
-          (ex_intro (fun y : b =>
-                       existsHash (fun x1 : a => k (x1, y)) = trueHash) x0 e1)).
-  exact (eq_sym e2).
-  intro.
-  pose (existsHashDef2' H).
-  elim a0.
-  intros.
-  elim H0.
-  intros.
-  pose (existsHashDef2' H2).
-  pose (proj1 a1).
-  elim e.
-  intros.
-  pose (ex_intro (fun x1 : a => k (x1, x0) = falseHash) x H3).
-  assert (not (exists (x1 : a), k (x1, x0) = trueHash)).
-  intro.
-  elim H4.
-  intros.
-  pose (existsHashDef1 (ex_intro (fun x0 : b => k (x1, x0) = trueHash) x0 H5)).
-  pose (existsHashDef1
-          (ex_intro (fun x1 : a =>
-                       existsHash (fun x0 : b =>
-                                     k (x1, x0)) = trueHash) x1 e1)).
-  rewrite H in e2.
-  exact (proj1 THash_not_eq (eq_sym e2)).
-  pose (ex_intro (fun x0 : b =>
-                    existsHash (fun x1 : a => k (x1, x0)) = falseHash)
-          x0 (existsHashDef2 (conj e0 H4))).
-  assert (not
-            (exists x0 : b, existsHash (fun x1 : a => k (x1, x0)) = trueHash)).
-  intro.
-  elim H5.
-  intros.
-  pose (existsHashDef1' H6).
-  elim e2.
-  intros.
-  pose (existsHashDef1 (ex_intro (fun x1 : b => k (x2, x1) = trueHash) x1 H7)).
-  pose (existsHashDef1
-          (ex_intro (fun x2 : a =>
-                       existsHash (fun x1 :
-                                     b => k (x2, x1)) = trueHash) x2 e3)).
-  rewrite H in e4.
-  exact (proj1 THash_not_eq (eq_sym e4)).
-  exact (eq_sym (existsHashDef2  (conj e1 H5))).
-  intro.
-  assert (forall y : b, existsHash (fun x : a => k (x, y)) = hash).
-  intro.
-  assert (forall x : a, k (x, y) = hash).
-  intro.
-  pose (existsHashDef3' H x).
-  exact (existsHashDef3' e y).
-  exact (existsHashDef3 H0).
-  exact (eq_sym (existsHashDef3 H0)).
-Qed.
+(* Weak Kleene ∧#. *)
+Parameter andHash : T# -> T# -> T#.
+Notation "A ∧# B" := (andHash A B) (at level 60, right associativity).
+Axiom andHashDef1 : forall (x : T#), (x ∧# # = #) /\ (# ∧# x = #).
+Axiom andHashDef2 : (⊤# ∧# ⊥# = ⊥#) /\ (⊥# ∧# ⊤# = ⊥#) /\ (⊥# ∧# ⊥# = ⊥#).
+Axiom andHashDef3 : ⊤# ∧# ⊤# = ⊤#.
 
-(* Weak Kleene ∧, i.e., ∧#. *)
-Parameter andHash : THash -> THash -> THash.
-Axiom andHashDef1 : forall (x : THash),
-    andHash x hash = hash /\ andHash hash x = hash.
-Axiom andHashDef2 : andHash trueHash falseHash = falseHash /\
-                      andHash falseHash trueHash = falseHash /\
-                      andHash falseHash falseHash = falseHash.
-Axiom andHashDef3 : andHash trueHash trueHash = trueHash.
-
-Lemma andHash_comm : forall (x y : THash), andHash x y = andHash y x.
+Lemma andHash_comm : forall (x y : T#), x ∧# y = y ∧# x.
 Proof.
   intros.
   case_eq x.
@@ -186,8 +119,8 @@ Proof.
   rewrite (proj1 (proj2 andHashDef2)).
   trivial.
   intros.
-  rewrite (proj1 (andHashDef1 trueHash)).
-  rewrite (proj2 (andHashDef1 trueHash)).
+  rewrite (proj1 (andHashDef1 ⊤#)).
+  rewrite (proj2 (andHashDef1 ⊤#)).
   trivial.
   intro.
   case_eq y.
@@ -198,25 +131,24 @@ Proof.
   intro.
   trivial.
   intro.
-  rewrite (proj1 (andHashDef1 falseHash)).
-  rewrite (proj2 (andHashDef1 falseHash)).
+  rewrite (proj1 (andHashDef1 ⊥#)).
+  rewrite (proj2 (andHashDef1 ⊥#)).
   trivial.
   intro.
   case_eq y.
   intro.
-  rewrite (proj1 (andHashDef1 trueHash)).
-  rewrite (proj2 (andHashDef1 trueHash)).
+  rewrite (proj1 (andHashDef1 ⊤#)).
+  rewrite (proj2 (andHashDef1 ⊤#)).
   trivial.
   intro.
-  rewrite (proj1 (andHashDef1 falseHash)).
-  rewrite (proj2 (andHashDef1 falseHash)).
+  rewrite (proj1 (andHashDef1 ⊥#)).
+  rewrite (proj2 (andHashDef1 ⊥#)).
   trivial.
   intro.
   trivial.
 Qed.
   
-Lemma andHash_assoc : forall (x y z : THash),
-    andHash x (andHash y z) = andHash (andHash x y) z.
+Lemma andHash_assoc : forall (x y z : T#), x ∧# (y ∧# z) = (x ∧# y) ∧# z.
 Proof.
   intros.
   case_eq x. case_eq y. case_eq z.
@@ -227,7 +159,7 @@ Proof.
   repeat rewrite (proj1 andHashDef2). trivial.
   intros.
   rewrite andHashDef3.
-  repeat rewrite (proj1 (andHashDef1 trueHash)). trivial.
+  repeat rewrite (proj1 (andHashDef1 ⊤#)). trivial.
   intros.
   case_eq z.
   intros.
@@ -240,22 +172,22 @@ Proof.
   rewrite (proj2 (proj2 andHashDef2)). trivial.
   intro.
   rewrite (proj1 andHashDef2).
-  repeat rewrite (proj1 (andHashDef1 falseHash)).
-  rewrite (proj1 (andHashDef1 trueHash)). trivial.
+  repeat rewrite (proj1 (andHashDef1 ⊥#)).
+  rewrite (proj1 (andHashDef1 ⊤#)). trivial.
   intros.
   case_eq z.
   intros.
-  rewrite (proj1 (andHashDef1 trueHash)).
-  repeat rewrite (proj2 (andHashDef1 trueHash)).
-  rewrite (proj1 (andHashDef1 trueHash)). trivial.
+  rewrite (proj1 (andHashDef1 ⊤#)).
+  repeat rewrite (proj2 (andHashDef1 ⊤#)).
+  rewrite (proj1 (andHashDef1 ⊤#)). trivial.
   intro.
-  rewrite (proj2 (andHashDef1 falseHash)).
-  rewrite (proj1 (andHashDef1 trueHash)).
-  rewrite (proj2 (andHashDef1 falseHash)). trivial.
+  rewrite (proj2 (andHashDef1 ⊥#)).
+  rewrite (proj1 (andHashDef1 ⊤#)).
+  rewrite (proj2 (andHashDef1 ⊥#)). trivial.
   intro.
-  rewrite (proj2 (andHashDef1 hash)).
-  rewrite (proj1 (andHashDef1 trueHash)).
-  rewrite (proj2 (andHashDef1 hash)). trivial.
+  rewrite (proj2 (andHashDef1 #)).
+  rewrite (proj1 (andHashDef1 ⊤#)).
+  rewrite (proj2 (andHashDef1 #)). trivial.
   case_eq y.
   case_eq z.
   intros.
@@ -266,9 +198,9 @@ Proof.
   rewrite (proj1 andHashDef2).
   repeat rewrite (proj2 (proj2 andHashDef2)). trivial.
   intros.
-  rewrite (proj1 (andHashDef1 trueHash)).
+  rewrite (proj1 (andHashDef1 ⊤#)).
   rewrite (proj1 (proj2 andHashDef2)).
-  repeat rewrite (proj1 (andHashDef1 falseHash)). trivial.
+  repeat rewrite (proj1 (andHashDef1 ⊥#)). trivial.
   intros.
   case_eq z.
   intros.
@@ -279,59 +211,58 @@ Proof.
   repeat rewrite (proj2 (proj2 andHashDef2)). trivial.
   intro.
   rewrite (proj2 (proj2 andHashDef2)).
-  repeat rewrite (proj1 (andHashDef1 falseHash)). trivial.
+  repeat rewrite (proj1 (andHashDef1 ⊥#)). trivial.
   intros.
   case_eq z.
   intro.
-  rewrite (proj1 (andHashDef1 falseHash)).
-  repeat rewrite (proj2 (andHashDef1 trueHash)).
-  rewrite (proj1 (andHashDef1 falseHash)). trivial.
+  rewrite (proj1 (andHashDef1 ⊥#)).
+  repeat rewrite (proj2 (andHashDef1 ⊤#)).
+  rewrite (proj1 (andHashDef1 ⊥#)). trivial.
   intro.
-  rewrite (proj1 (andHashDef1 falseHash)).
-  rewrite (proj2 (andHashDef1 falseHash)).
-  rewrite (proj1 (andHashDef1 falseHash)). trivial.
+  rewrite (proj1 (andHashDef1 ⊥#)).
+  rewrite (proj2 (andHashDef1 ⊥#)).
+  rewrite (proj1 (andHashDef1 ⊥#)). trivial.
   intro.
-  rewrite (proj1 (andHashDef1 hash)).
-  repeat rewrite (proj1 (andHashDef1 falseHash)).
-  rewrite (proj1 (andHashDef1 hash)). trivial.
+  rewrite (proj1 (andHashDef1 #)).
+  repeat rewrite (proj1 (andHashDef1 ⊥#)).
+  rewrite (proj1 (andHashDef1 #)). trivial.
   case_eq y.
   case_eq z.
   intros.
   rewrite andHashDef3.
-  repeat rewrite (proj2 (andHashDef1 trueHash)). trivial.
+  repeat rewrite (proj2 (andHashDef1 ⊤#)). trivial.
   intros.
   rewrite (proj1 andHashDef2).
-  rewrite (proj2 (andHashDef1 trueHash)). trivial.
+  rewrite (proj2 (andHashDef1 ⊤#)). trivial.
   intros.
-  rewrite (proj2 (andHashDef1 trueHash)).
-  rewrite (proj1 (andHashDef1 trueHash)). trivial.
+  rewrite (proj2 (andHashDef1 ⊤#)).
+  rewrite (proj1 (andHashDef1 ⊤#)). trivial.
   case_eq z.
   intros.
-  rewrite (proj2 (andHashDef1 falseHash)).
+  rewrite (proj2 (andHashDef1 ⊥#)).
   rewrite (proj1 (proj2 andHashDef2)).
-  rewrite (proj2 (andHashDef1 falseHash)).
-  rewrite (proj2 (andHashDef1 trueHash)). trivial.
+  rewrite (proj2 (andHashDef1 ⊥#)).
+  rewrite (proj2 (andHashDef1 ⊤#)). trivial.
   intros.
   rewrite (proj2 (proj2 andHashDef2)).
-  repeat rewrite (proj2 (andHashDef1 falseHash)). trivial.
+  repeat rewrite (proj2 (andHashDef1 ⊥#)). trivial.
   intros.
-  rewrite (proj2 (andHashDef1 falseHash)).
-  rewrite (proj1 (andHashDef1 falseHash)). trivial.
+  rewrite (proj2 (andHashDef1 ⊥#)).
+  rewrite (proj1 (andHashDef1 ⊥#)). trivial.
   case_eq z.
   intros.
-  rewrite (proj2 (andHashDef1 trueHash)).
-  repeat rewrite (proj2 (andHashDef1 hash)).
-  rewrite (proj2 (andHashDef1 trueHash)). trivial.
+  rewrite (proj2 (andHashDef1 ⊤#)).
+  repeat rewrite (proj2 (andHashDef1 #)).
+  rewrite (proj2 (andHashDef1 ⊤#)). trivial.
   intros.
-  rewrite (proj2 (andHashDef1 falseHash)).
-  repeat rewrite (proj2 (andHashDef1 hash)).
-  rewrite (proj2 (andHashDef1 falseHash)). trivial.
+  rewrite (proj2 (andHashDef1 ⊥#)).
+  repeat rewrite (proj2 (andHashDef1 #)).
+  rewrite (proj2 (andHashDef1 ⊥#)). trivial.
   intros.
-  repeat rewrite (proj2 (andHashDef1 hash)). trivial.
+  repeat rewrite (proj2 (andHashDef1 #)). trivial.
 Qed.
  
-Lemma andHash_is_true : forall {x  y : THash},
-    andHash x y = trueHash -> x = trueHash /\ y = trueHash.
+Lemma andHash_is_true : forall {x  y : T#}, x ∧# y = ⊤# -> (x = ⊤# /\ y = ⊤#).
 Proof.
   intros.
   case_eq x.
@@ -346,7 +277,7 @@ Proof.
   intros.
   rewrite H0 in H.
   rewrite H1 in H.
-  rewrite (proj1 (andHashDef1 trueHash)) in H.
+  rewrite (proj1 (andHashDef1 ⊤#)) in H.
   exact (conj eq_refl H).
   intros.
   rewrite H0 in H.
@@ -361,7 +292,7 @@ Proof.
   exact (conj H H).
   intros.
   rewrite H1 in H.
-  rewrite (proj1 (andHashDef1 falseHash)) in H.
+  rewrite (proj1 (andHashDef1 ⊥#)) in H.
   pose (proj1 (proj2 THash_not_eq) H).
   inversion f.
   intros.
@@ -369,22 +300,21 @@ Proof.
   case_eq y.
   intros.
   rewrite H1 in H.
-  rewrite (proj2 (andHashDef1 trueHash)) in H.
+  rewrite (proj2 (andHashDef1 ⊤#)) in H.
   pose (proj1 (proj2 THash_not_eq) H).
   inversion f.
   intros.
   rewrite H1 in H.
-  rewrite (proj2 (andHashDef1 falseHash)) in H.
+  rewrite (proj2 (andHashDef1 ⊥#)) in H.
   pose (proj1 (proj2 THash_not_eq) H).
   inversion f.
   intros.
   rewrite H1 in H.
-  rewrite (proj1 (andHashDef1 hash)) in H.
+  rewrite (proj1 (andHashDef1 #)) in H.
   exact (conj H H).
 Qed.
 
-Lemma andHash_is_false1 : forall {x y : THash},
-    andHash x y = falseHash -> x = falseHash \/ y = falseHash.
+Lemma andHash_is_false1 : forall {x y : T#}, x ∧# y = ⊥# -> (x = ⊥# \/ y = ⊥#).
 Proof.
   intros.
   case_eq x.
@@ -401,7 +331,7 @@ Proof.
   intro.
   rewrite H0 in H.
   rewrite H1 in H.
-  rewrite (proj1 (andHashDef1 trueHash)) in H.
+  rewrite (proj1 (andHashDef1 ⊤#)) in H.
   pose (proj2 (proj2 THash_not_eq) H).
   inversion f.
   intro.
@@ -411,7 +341,7 @@ Proof.
   intro.
   rewrite H0 in H.
   rewrite H1 in H.
-  rewrite (proj2 (andHashDef1 trueHash)) in H.
+  rewrite (proj2 (andHashDef1 ⊤#)) in H.
   pose (proj2 (proj2 THash_not_eq) H).
   inversion f.
   intro.
@@ -419,17 +349,15 @@ Proof.
   intro.
   rewrite H0 in H.
   rewrite H1 in H.
-  rewrite (proj1 (andHashDef1 hash)) in H.
+  rewrite (proj1 (andHashDef1 #)) in H.
   pose (proj2 (proj2 THash_not_eq) H).
   inversion f.
 Qed.
 
-Lemma andHash_is_false2 : forall {x y : THash},
-    andHash x y = falseHash ->
-    (x = trueHash \/ x = falseHash) /\ (y = trueHash \/ y = falseHash).
+Lemma andHash_is_false2 :
+  forall {x y : T#}, x ∧# y = ⊥# -> (x = ⊤# \/ x = ⊥#) /\ (y = ⊤# \/ y = ⊥#).
 Proof.
-  assert (forall (x y : THash),
-             andHash x y = falseHash -> x = trueHash \/ x = falseHash). intros.
+  assert (forall (x y : T#), x ∧# y = ⊥# -> (x = ⊤# \/ x = ⊥#)). intros.
   case_eq x. intro.
   left. trivial.
   intro.
@@ -446,8 +374,7 @@ Proof.
   exact (H y x H0).
 Qed.
  
-Lemma andHash_is_hash : forall {x y : THash},
-    andHash x y = hash -> x = hash \/ y = hash.
+Lemma andHash_is_hash : forall {x y : T#}, x ∧# y = # -> (x = # \/ y = #).
 Proof.
   intros.
   case_eq x.
@@ -490,116 +417,80 @@ Proof.
   trivial.
 Qed.
 
-Parameter delt : T -> THash.
-Axiom deltDef : delt true = trueHash /\ delt false = hash.
-
-Lemma delt_inj : forall {x y : T}, delt x = delt y -> x = y.
+Lemma andHash_existsHash_comm :
+  forall {a : Set} (φ : a -> T#) (p : T#),
+    (∃# φ) ∧# p = ∃# (fun x : a => φ x ∧# p).
 Proof.
   intros.
-  case_eq x.
-  case_eq y.
-  intros.
-  trivial.
-  intros.
-  rewrite H0 in H.
-  rewrite H1 in H.
-  rewrite (proj1 deltDef) in H.
-  rewrite (proj2 deltDef) in H.
-  pose (proj1 (proj2 THash_not_eq) (eq_sym H)).
-  inversion f.
-  case_eq x.
-  intro.
-  case_eq y.
-  intros.
-  exact (eq_sym H2).
-  intros.
-  trivial.
-  intros.
-  case_eq y.
-  intros.
-  rewrite H0 in H.
-  rewrite H2 in H.
-  rewrite (proj1 deltDef) in H.
-  rewrite (proj2 deltDef) in H.
-  pose (proj1 (proj2 THash_not_eq) H).
-  inversion f.
-  intro.
-  trivial.
-Qed.
-
-Lemma andHash_existsHash_comm : forall {a : Set} (phi : a -> THash) (p : THash),
-    andHash (existsHash phi) p = existsHash (fun x : a => andHash (phi x) p).
-Proof.
-  intros.
-  case_eq (andHash (existsHash phi) p).
+  case_eq ((∃# φ) ∧# p).
   intro.
   pose (andHash_is_true H).
   pose (existsHashDef1' (proj1 a0)).
   elim e.
   intros.
   pose andHashDef3.
-  replace (andHash trueHash trueHash = trueHash) with
-    (andHash (phi x) trueHash = trueHash) in e0 by now (rewrite (eq_sym H0)).
-  replace (andHash (phi x) trueHash = trueHash) with
-    (andHash (phi x) p = trueHash) in e0 by now (rewrite (proj2 a0)).
+  replace (⊤# ∧# ⊤# = ⊤#) with
+    (φ x ∧# ⊤# = ⊤#) in e0 by now (rewrite (eq_sym H0)).
+  replace (φ x ∧# ⊤# = ⊤#) with
+    (φ x ∧# p = ⊤#) in e0 by now (rewrite (proj2 a0)).
   exact (eq_sym
            (existsHashDef1
-              (ex_intro (fun x0 : a => andHash (phi x0) p = trueHash) x e0))).
+              (ex_intro (fun x0 : a => (φ x0) ∧# p = ⊤#) x e0))).
   intro.
   pose (andHash_is_false1 H).
   elim o.
   intro.
   pose (existsHashDef2' H0).
-  assert (exists x : a, andHash (phi x) p = falseHash).
+  assert (exists x : a, (φ x) ∧# p = ⊥#).
   elim (proj1 a0).
   intros.
   case_eq p.
   intro.
   pose (proj1 (proj2 andHashDef2)).
-  replace (andHash falseHash trueHash = falseHash) with
-    (andHash (phi x) trueHash = falseHash) in e by now (rewrite (eq_sym H1)).
-  exact (ex_intro (fun x0 : a => andHash (phi x0) trueHash = falseHash) x e).
+  replace (andHash ⊥# ⊤# = ⊥#) with
+    (φ x ∧# ⊤# = ⊥#) in e by now (rewrite (eq_sym H1)).
+  exact (ex_intro (fun x0 : a => (φ x0) ∧# ⊤# = ⊥#) x e).
   intro.
   pose (proj2 (proj2 andHashDef2)).
-  replace (andHash falseHash falseHash = falseHash) with
-    (andHash (phi x) falseHash = falseHash) in e by now (rewrite (eq_sym H1)).
-  exact (ex_intro (fun x0 : a => andHash (phi x0) falseHash = falseHash) x e).
+  replace (⊥# ∧# ⊥# = ⊥#) with
+    (φ x ∧# ⊥# = ⊥#) in e by now (rewrite (eq_sym H1)).
+  exact (ex_intro (fun x0 : a => φ x0 ∧# ⊥# = ⊥#) x e).
   intro.
   pose H.
   rewrite H2 in e.
-  rewrite (proj1 (andHashDef1 (existsHash phi))) in e.
+  rewrite (proj1 (andHashDef1 (existsHash φ))) in e.
   pose (proj2 (proj2 THash_not_eq) e).
   inversion f.
-  assert (~ (exists x : a, andHash (phi x) p = trueHash)).
+  assert (~ (exists x : a, φ x ∧# p = ⊤#)).
   intro.
   elim H2.
   intros.
   exact (proj2 a0 (ex_intro
-                     (fun x => phi x = trueHash)
+                     (fun x => φ x = ⊤#)
                      x (proj1 (andHash_is_true H3)))).
   exact (eq_sym (existsHashDef2 (conj H1 H2))).
   intro.
   rewrite H0.
-  case_eq (existsHash phi). intro.
+  case_eq (existsHash φ). intro.
   pose (existsHashDef1' H1).
   elim e. intros.
   pose (proj1 andHashDef2).
   rewrite (eq_sym H2) in e0.
-  pose (ex_intro (fun x : a => andHash (phi x) falseHash = falseHash) x e0).
-  assert (~ exists x : a, andHash (phi x) falseHash = trueHash). intro.
+  pose (ex_intro (fun x : a => φ x ∧# ⊥# = ⊥#) x e0).
+  assert (~ exists x : a, φ x ∧# ⊥# = ⊤#). intro.
   elim H3. intros.
   exact (proj1 THash_not_eq
            (eq_sym (proj2 (andHash_is_true H4)))).
   exact (eq_sym (existsHashDef2 (conj e1 H3))).
   intro.
   pose (existsHashDef2' H1).
-  assert (exists x : a, andHash (phi x) falseHash = falseHash).
+  assert (exists x : a, (φ x) ∧# ⊥# = ⊥#).
   elim (proj1 a0). intros.
   pose (proj2 (proj2 andHashDef2)).
-  replace (andHash falseHash falseHash = falseHash) with
-    (andHash (phi x) falseHash = falseHash) in e by now (rewrite (eq_sym H2)).
-  exact (ex_intro (fun x0 : a => andHash (phi x0) falseHash = falseHash) x e).
-  assert (~ exists x : a, andHash (phi x) falseHash = trueHash). intro.
+  replace (⊥# ∧# ⊥# = ⊥#) with
+    (φ x ∧# ⊥# = ⊥#) in e by now (rewrite (eq_sym H2)).
+  exact (ex_intro (fun x0 : a => φ x0 ∧# ⊥# = ⊥#) x e).
+  assert (~ exists x : a, φ x ∧# ⊥# = ⊤#). intro.
   elim H3. intros.
   exact (proj1 THash_not_eq
            (eq_sym (proj2 (andHash_is_true H4)))).
@@ -614,76 +505,60 @@ Proof.
   pose (proj2 (proj2 THash_not_eq) H2).
   inversion f.
   intro.
-  assert (forall x : a, andHash (phi x) p = hash). intro.
+  assert (forall x : a, φ x ∧# p = #). intro.
   pose (andHash_is_hash H).
   elim o. intro.
   pose (existsHashDef3' H0 x).
   pose (proj2 (andHashDef1 p)).
-  replace (andHash hash p = hash) with
-    (andHash (phi x) p = hash) in e0 by now (rewrite (eq_sym e)).
+  replace (# ∧# p = #) with
+    (φ x ∧# p = #) in e0 by now (rewrite (eq_sym e)).
   exact e0.
   intro.
   rewrite H0.
-  exact (proj1 (andHashDef1 (phi x))).
+  exact (proj1 (andHashDef1 (φ x))).
   exact (eq_sym (existsHashDef3 H0)).
 Qed.
 
-Lemma existsHash_andHash_existsHash_andHash : forall {a b : Set}
-                                                     (m : b -> THash)
-                                                     (n : a -> b -> THash)
-                                                     (o : a -> THash),
-    existsHash (fun x : a =>
-                  andHash (existsHash (fun y : b =>
-                                         andHash (m y) (n x y))) (o x)) =
-      existsHash (fun y : b =>
-                    andHash (m y) (existsHash (fun x : a =>
-                                                 andHash (n x y) (o x)))).
+Lemma existsHash_andHash_existsHash_andHash :
+  forall {a b : Set}
+         (m : b -> T#)
+         (n : a -> b -> T#)
+         (o : a -> T#),
+    (∃# (fun x : a => (∃# (fun y : b => m y ∧# n x y)) ∧# o x)) =
+      (∃# (fun y : b => m y ∧# (∃# (fun x : a => n x y ∧# o x)))).
 Proof.
   intros.
-  case_eq (existsHash (fun x : a =>
-                         andHash (existsHash (fun y : b =>
-                                                andHash (m y)
-                                                  (n x y))) (o x))).
+  case_eq (∃# (fun x : a => (∃# (fun y : b => m y ∧# n x y)) ∧# o x)).
   intros.
   pose (existsHashDef1' H).
   elim e. intros.
-  rewrite (andHash_existsHash_comm (fun y : b =>
-                                      andHash (m y) (n x y))) in H0.
+  rewrite (andHash_existsHash_comm (fun y : b => m y ∧# n x y)) in H0.
   pose (existsHashDef1' H0).
   elim e0. intros.
   pose (andHash_is_true H1).
   pose (andHash_is_true (proj1 a0)).
-  assert (exists (x1 : a), andHash (n x1 x0) (o x1) = trueHash).
+  assert (exists (x1 : a), n x1 x0 ∧# o x1 = ⊤#).
   pose andHashDef3.
-  replace (andHash trueHash trueHash = trueHash) with
-    (andHash (n x x0) trueHash = trueHash) in e1 by now (rewrite (proj2 a1)).
-  replace  (andHash (n x x0) trueHash = trueHash) with
-    (andHash (n x x0) (o x) = trueHash) in e1 by now (rewrite (proj2 a0)).
-  exact (ex_intro (fun x1 : a => andHash (n x1 x0) (o x1) = trueHash) x e1).
+  replace (⊤# ∧# ⊤# = ⊤#) with (n x x0 ∧# ⊤# = ⊤#) in e1 by
+      now (rewrite (proj2 a1)).
+  replace  (n x x0 ∧# ⊤# = ⊤#) with (n x x0 ∧# o x = ⊤#) in e1 by
+      now (rewrite (proj2 a0)).
+  exact (ex_intro (fun x1 : a => n x1 x0 ∧# o x1 = ⊤#) x e1).
   pose (existsHashDef1 H2).
   pose andHashDef3.
-  replace (andHash trueHash trueHash = trueHash) with
-    (andHash trueHash (existsHash (fun x1 : a =>
-                                     andHash (n x1 x0) (o x1))) = trueHash)
-    in e2 by now (rewrite (eq_sym e1)).
-  replace (andHash trueHash (existsHash (fun x1 : a =>
-                                           andHash (n x1 x0)
-                                             (o x1))) = trueHash) with
-    (andHash (m x0) (existsHash (fun x1 : a =>
-                                   andHash (n x1 x0) (o x1))) = trueHash)
-    in e2 by now (rewrite (eq_sym (proj1 a1))).
+  replace (⊤# ∧# ⊤# = ⊤#) with
+    (⊤# ∧# (∃# (fun x1 : a => n x1 x0 ∧# o x1)) = ⊤#) in e2 by
+      now (rewrite (eq_sym e1)).
+  replace (⊤# ∧# (∃# (fun x1 : a => n x1 x0 ∧# o x1)) = ⊤#) with
+    (m x0 ∧# (∃# (fun x1 : a => n x1 x0 ∧# o x1)) = ⊤#) in e2 by
+      now (rewrite (eq_sym (proj1 a1))).
   exact (eq_sym
-           (existsHashDef1 (ex_intro (fun y : b =>
-                                        andHash (m y)
-                                          (existsHash (fun x1 : a =>
-                                                         andHash (n x1 y)
-                                                           (o x1))) =
-                                          trueHash)
-                              x0 e2))).
+           (existsHashDef1
+              (ex_intro
+                 (fun y : b => m y ∧# (∃# (fun x1 : a => n x1 y ∧# o x1)) = ⊤#)
+                 x0 e2))).
   intro.
-  case_eq (existsHash (fun y : b =>
-                         andHash (m y)
-                           (existsHash (fun x : a => andHash (n x y) (o x))))).
+  case_eq (∃# (fun y : b => m y ∧# (∃# (fun x : a => n x y ∧# o x)))).
   intro.
   pose (existsHashDef1' H0).
   elim e. intros.
@@ -692,38 +567,28 @@ Proof.
   elim e0. intros.
   pose (andHash_is_true H2).
   pose andHashDef3.
-  replace (andHash trueHash) with
-    (andHash (m x)) in e1 by now (rewrite (eq_sym (proj1 a0))).
-  replace (andHash (m x) trueHash) with
-    (andHash (m x) (n x0 x)) in e1 by now (rewrite (eq_sym (proj1 a1))).
-  pose (existsHashDef1 (ex_intro (fun y : b =>
-                                    andHash (m y) (n x0 y) = trueHash) x e1)).
+  replace (⊤# ∧# ⊤#) with (m x ∧# ⊤#) in e1 by
+      now (rewrite (eq_sym (proj1 a0))).
+  replace (m x ∧# ⊤#) with (m x ∧# n x0 x) in e1 by
+      now (rewrite (eq_sym (proj1 a1))).
+  pose (existsHashDef1 (ex_intro (fun y : b => m y ∧# n x0 y = ⊤#) x e1)).
   pose andHashDef3.
-  replace (andHash trueHash) with
-    (andHash (existsHash (fun y : b => andHash (m y) (n x0 y)))) in e3 by
+  replace (⊤# ∧# ⊤#) with ((∃# (fun y : b => m y ∧# n x0 y)) ∧# ⊤#) in e3 by
       now (rewrite (eq_sym e2)).
-  replace (andHash (existsHash (fun y : b =>
-                                  andHash (m y) (n x0 y))) trueHash) with
-    (andHash (existsHash (fun y : b =>
-                            andHash (m y) (n x0 y))) (o x0))
-    in e3 by
+  replace ((∃# (fun y : b => m y ∧# n x0 y)) ∧# ⊤#) with
+    ((∃# (fun y : b => m y ∧# n x0 y)) ∧# o x0) in e3 by
       now (rewrite (eq_sym (proj2 a1))).
   rewrite (existsHashDef1
              (ex_intro
-                (fun x : a =>
-                   andHash (existsHash
-                              (fun y : b =>
-                                 andHash (m y) (n x y))) (o x) = trueHash)
+                (fun x : a => (∃# (fun y : b => m y ∧# n x y)) ∧# o x = ⊤#)
                 x0 e3)) in H.
   exact (eq_sym H).
   trivial.
   intro.
-  assert (forall x : a,
-             andHash (existsHash (fun y : b =>
-                                    andHash (m y) (n x y))) (o x) = hash).
+  assert (forall x : a, (∃# (fun y : b => m y ∧# n x y)) ∧# o x = #).
   intro.
   pose (existsHashDef3' H0).
-  case_eq (existsHash (fun y : b => andHash (m y) (n x y))). intro.
+  case_eq (∃# (fun y : b => m y ∧# n x y)). intro.
   pose (existsHashDef1' H1).
   elim e0. intros.
   pose (andHash_is_hash (e x0)). elim o0. intro.
@@ -751,7 +616,7 @@ Proof.
   inversion f.
   intro.
   rewrite H4.
-  apply (proj1 (andHashDef1 falseHash)).
+  apply (proj1 (andHashDef1 ⊥#)).
   intro.
   apply (proj2 (andHashDef1 (o x))).
   pose (existsHashDef2' H).
@@ -767,16 +632,12 @@ Proof.
   exact H3.
   intro.
   rewrite H3 in H2.
-  rewrite (proj1 (andHashDef1 (existsHash (fun y : b =>
-                                             andHash (m y) (n x y))))) in H2.
+  rewrite (proj1 (andHashDef1 (∃# (fun y : b => m y ∧# n x y)))) in H2.
   exact (eq_sym H2).
   intro.
-  assert (forall (y : b),
-             andHash (m y)
-               (existsHash (fun x : a =>
-                              andHash (n x y) (o x))) = hash). intro.
+  assert (forall (y : b), m y ∧#  (∃# (fun x : a => n x y ∧# o x)) = #). intro.
   case_eq (m y). intro.
-  assert (forall (x : a), andHash (n x y) (o x) = hash). intro.
+  assert (forall (x : a), n x y ∧# o x = #). intro.
   pose (existsHashDef3' H x).
   pose (andHash_is_hash e).
   elim o0. intro.
@@ -793,9 +654,9 @@ Proof.
   rewrite H1.
   exact (proj1 (andHashDef1 (n x y))).
   rewrite (existsHashDef3 H1).
-  exact (proj1 (andHashDef1 trueHash)).
+  exact (proj1 (andHashDef1 ⊤#)).
   intro.
-    assert (forall (x : a), andHash (n x y) (o x) = hash). intro.
+  assert (forall (x : a), n x y ∧# o x = #). intro.
   pose (existsHashDef3' H x).
   pose (andHash_is_hash e).
   elim o0. intro.
@@ -812,40 +673,45 @@ Proof.
   rewrite H1.
   exact (proj1 (andHashDef1 (n x y))).
   rewrite (existsHashDef3 H1).
-  exact (proj1 (andHashDef1 falseHash)).
+  exact (proj1 (andHashDef1 ⊥#)).
   intro.
-  exact (proj2 (andHashDef1 (existsHash (fun x : a => andHash (n x y) (o x))))).
+  exact (proj2 (andHashDef1 (∃# (fun x : a => n x y ∧# o x)))).
   exact (eq_sym (existsHashDef3 H0)).
 Qed.
-  
-Lemma delt_true : forall {x : T}, delt x = trueHash -> x = true.
+
+Parameter δ : T -> T#.
+(* Notation "δ " := δ (at level 85, right associativity). *)
+Axiom δDef : δ ⊤ = ⊤# /\ δ ⊥ = #.
+
+Lemma δ_true : forall {x : T}, δ x = ⊤# -> x = true.
 Proof.
   intros.
   case_eq x. intro.
   trivial.
   intro.
   rewrite H0 in H.
-  rewrite (proj2 deltDef) in H.
+  rewrite (proj2 δDef) in H.
   pose (proj1 (proj2 THash_not_eq) H).
   inversion f.
 Qed.
 
 Parameter eqHash : forall {a : Set}, a -> a -> T.
-Axiom eqHashRefl1 : forall {a : Set} {x y : a}, x = y -> eqHash x y = true.
-Axiom eqHashRefl2 : forall {a : Set} {x y : a}, eqHash x y = true -> x = y.
+Notation "x ≡ y" := (eqHash x y) (at level 80, right associativity).
+Axiom eqHashRefl1 : forall {a : Set} {x y : a}, x = y -> (x ≡ y) = ⊤.
+Axiom eqHashRefl2 : forall {a : Set} {x y : a}, (x ≡ y) = ⊤ -> x = y.
 
-Lemma eqHashRefl1_converse : forall {a : Set} {x y : a},
-    ~ (x = y) -> eqHash x y = false.
+Lemma eqHashRefl1_converse :
+  forall {a : Set} {x y : a}, ~ (x = y) -> (x ≡ y) = ⊥.
 Proof.
   intros.
-  case_eq (eqHash x y). intro.
+  case_eq (x ≡ y). intro.
   pose (H (eqHashRefl2 H0)).
   inversion f.
   trivial.
 Qed.
 
-Lemma eqHashRefl2_converse : forall {a : Set} {x y : a},
-    eqHash x y = false -> ~ (x = y).
+Lemma eqHashRefl2_converse :
+  forall {a : Set} {x y : a}, (x ≡ y) = ⊥ -> ~ (x = y).
 Proof.
   intros.
   intro.
@@ -854,11 +720,11 @@ Proof.
   exact (T_not_eq H).
 Qed.
 
-Lemma eqHash_comm : forall {a : Set} (x y : a), eqHash x y = eqHash y x.
+Lemma eqHash_comm : forall {a : Set} (x y : a), (x ≡ y) = (y ≡ x).
 Proof.
   intros.
-  case_eq (eqHash x y).
-  case_eq (eqHash y x).
+  case_eq (x ≡ y).
+  case_eq (y ≡ x).
   intros. trivial.
   intros.
   pose (eqHashRefl2_converse H).
@@ -875,61 +741,56 @@ Proof.
   intro. trivial.
 Qed.
 
-Theorem delt_elim : forall {a : Set} (v : a) (phi : a -> THash),
-    existsHash (fun (x : a) => andHash (delt (eqHash x v)) (phi x)) = phi v.
+Lemma δElim :
+  forall {a : Set} (v : a) (φ : a -> T#),
+    (∃# (fun (x : a) => δ (x ≡ v) ∧# φ x)) = φ v.
 Proof.
   intros.
-  case_eq (phi v).
+  case_eq (φ v).
   intro. apply eq_sym in H.
   pose andHashDef3.
-  replace (andHash trueHash trueHash = trueHash) with
-    (andHash trueHash (phi v) = trueHash) in e by now (rewrite H).
-  pose (proj1 deltDef).
-  replace (delt true = trueHash) with
-    (delt (eqHash v v) = trueHash) in e0 by
+  replace (⊤# ∧# ⊤# = ⊤#) with (⊤# ∧# φ v = ⊤#) in e by now (rewrite H).
+  pose (proj1 δDef).
+  replace (δ ⊤ = ⊤#) with (δ (v ≡ v) = ⊤#) in e0 by
       now (rewrite (eq_sym (eqHashRefl1 (eq_refl v)))).
   apply eq_sym in e0.
-  replace (andHash trueHash (phi v) = trueHash) with
-    (andHash (delt (eqHash v v)) (phi v) = trueHash) in e by now (rewrite e0).
-  pose (ex_intro
-          (fun x : a => andHash (delt (eqHash x v)) (phi x) = trueHash) v e).
+  replace (⊤# ∧# φ v = ⊤#) with (δ (v ≡ v) ∧# φ v = ⊤#) in e by
+      now (rewrite e0).
+  pose (ex_intro (fun x : a => δ (x ≡ v) ∧# φ x = ⊤#) v e).
   exact (existsHashDef1 e1).
   intro. apply eq_sym in H.
   pose (proj1 andHashDef2).
-  replace (andHash trueHash falseHash = falseHash) with
-    (andHash trueHash (phi v) = falseHash) in e by now (rewrite H).
-  pose (proj1 deltDef).
-  replace (delt true = trueHash) with
-    (delt (eqHash v v) = trueHash) in e0 by
+  replace (⊤# ∧# ⊥# = ⊥#) with (⊤# ∧# φ v = ⊥#) in e by now (rewrite H).
+  pose (proj1 δDef).
+  replace (δ ⊤ = ⊤#) with (δ (v ≡ v) = ⊤#) in e0 by
       now (rewrite (eq_sym (eqHashRefl1 (eq_refl v)))).
   apply eq_sym in e0.
-  replace (andHash trueHash (phi v) = falseHash) with
-    (andHash (delt (eqHash v v)) (phi v) = falseHash) in e by now (rewrite e0).
-  pose (ex_intro
-          (fun x : a => andHash (delt (eqHash x v)) (phi x) = falseHash) v e).
-  assert (~ (exists x : a, andHash (delt (eqHash x v)) (phi x) = trueHash)).
+  replace (⊤# ∧# φ v = ⊥#) with (δ (v ≡ v) ∧# φ v = ⊥#) in e by
+      now (rewrite e0).
+  pose (ex_intro (fun x : a => δ (x ≡ v) ∧# φ x = ⊥#) v e).
+  assert (~ (exists x : a, δ (x ≡ v) ∧# φ x = ⊤#)).
   intro.
   elim H0.
   intros.
   pose (andHash_is_true H1).
   pose (proj1 a0).
-  pose (eqHashRefl2 (delt_true e2)).
+  pose (eqHashRefl2 (δ_true e2)).
   pose (proj2 a0).
   rewrite e3 in e4.
   rewrite e4 in H.
   exact (proj1 THash_not_eq (eq_sym H)).
   exact (existsHashDef2 (conj e1 H0)).
   intros.
-  assert (forall (x : a), andHash (delt (eqHash x v)) (phi x) = hash).
+  assert (forall (x : a), δ (x ≡ v) ∧# φ x = #).
   intro.
   case_eq (eqHash x v). intro.
   rewrite (eqHashRefl2 H0).
   rewrite H.
-  rewrite (proj1 (andHashDef1 (delt true))).
+  rewrite (proj1 (andHashDef1 (δ ⊤))).
   trivial.
   intro.
-  rewrite (proj2 deltDef).
-  rewrite (proj2 (andHashDef1 (phi x))).
+  rewrite (proj2 δDef).
+  rewrite (proj2 (andHashDef1 (φ x))).
   trivial.
   exact (existsHashDef3 H0).
 Qed.
@@ -964,86 +825,69 @@ Definition monad
   (bind : forall (a b : Set), m a -> (a -> m b) -> m b) :=
   monad_left_id m eta bind /\ monad_right_id m eta bind /\ monad_assoc m bind.
 
-(* The functor S#, defined as S# α = α → t#. *)
+(* The functor S#, defined as S# α = α -> t#. *)
 Definition SHash (a : Set) := a -> THash.
-Definition etaHash (a : Set) (x : a) : SHash a :=
-  fun y : a => delt (eqHash y x).
+Notation "S#" := SHash.
+Definition etaHash (a : Set) (x : a) : S# a := fun y : a => δ (y ≡ x).
+Notation "η#" := etaHash.
 Definition bindHash (a b : Set) (m : SHash a) (k : a -> SHash b) : SHash b :=
-  fun y : b => existsHash (fun x : a => andHash (m x) (k x y)).
+  fun y : b => (∃# (fun x : a => m x ∧# k x y)).
+Notation "⋆#" := bindHash.
+Notation "m ⋆# k" := (bindHash m k) (at level 190, left associativity).
 
 (* We need functional extensionality (a.k.a. η-expansion). *)
 Axiom functional_extensionality: forall {a b} (f g : a -> b),
     (forall x, f x = g x) -> f = g.
 
 (* The grand finale! *)
-Theorem SHash_is_a_monad : monad SHash etaHash bindHash.
+Theorem SHash_is_a_monad : monad S# η# ⋆#.
 Proof.
   split.
   unfold monad_left_id. unfold bindHash. unfold etaHash.
   intros.
-  pose (functional_extensionality (fun y : b =>
-                                     existsHash (fun x0 : a =>
-                                                   andHash (delt (eqHash x0 x))
-                                                     (k x0 y))) (k x)).
+  pose (functional_extensionality
+          (fun y : b => ∃# (fun x0 : a => δ (x0 ≡ x) ∧# k x0 y))
+          (k x)).
   assert (forall x0 : b,
              (fun y : b =>
-                existsHash (fun x1 : a =>
-                              andHash (delt (eqHash x1 x)) (k x1 y))) x0 =
-               k x x0).
+                ∃# (fun x1 : a => (δ (x1 ≡ x)) ∧# k x1 y)) x0 = k x x0).
   intro.
-  rewrite (delt_elim x (fun x' : a => k x' x0)). trivial.
+  rewrite (δElim x (fun x' : a => k x' x0)). trivial.
   exact (e H).
   split.
   unfold monad_right_id. unfold bindHash. unfold etaHash.
   intros.
   pose (functional_extensionality
-          (fun y : a =>
-             existsHash (fun x : a => andHash (m' x) (delt (eqHash y x)))) m').
+          (fun y : a => ∃# (fun x : a => m' x ∧# δ (y ≡ x)))
+          m').
   assert (forall x : a,
-             existsHash (fun x0 : a =>
-                           andHash (m' x0) (delt (eqHash x x0))) = m' x).
+             (∃# (fun x0 : a => m' x0 ∧# δ (x ≡ x0))) = m' x).
   intro.
-  assert ((fun x0 : a => andHash (m' x0) (delt (eqHash x x0))) =
-            fun x0 : a => andHash (delt (eqHash x0 x)) (m' x0)).
+  assert
+    ((fun x0 : a => m' x0 ∧# δ (x ≡ x0)) = (fun x0 : a => δ (x0 ≡ x) ∧# m' x0)).
   pose (functional_extensionality
-          (fun x0 : a =>
-             andHash (m' x0)
-               (delt (eqHash x x0))) (fun x0 : a =>
-                                        andHash (delt (eqHash x0 x)) (m' x0))).
-  assert (forall x0 : a,
-             andHash (m' x0)
-               (delt (eqHash x x0)) = andHash (delt (eqHash x0 x)) (m' x0)).
+          (fun x0 : a => m' x0 ∧# δ (x ≡ x0))
+          (fun x0 : a => δ (x0 ≡ x) ∧# m' x0)).
+  assert (forall x0 : a, m' x0 ∧# δ (x ≡ x0) = δ (x0 ≡ x) ∧# m' x0).
   intro.
   rewrite (eqHash_comm x x0).
-  exact (andHash_comm (m' x0) (delt (eqHash x0 x))).
+  exact (andHash_comm (m' x0) (δ (x0 ≡ x))).
   exact (e0 H).
   rewrite H.
-  rewrite (delt_elim x m'). trivial.
+  rewrite (δElim x m'). trivial.
   exact (e H).
   unfold monad_assoc. unfold bindHash.
   intros.
   pose (functional_extensionality
           (fun y : c =>
-             existsHash (fun x : b =>
-                           andHash
-                             (existsHash (fun x0 : a =>
-                                            andHash (m' x0)
-                                              (n x0 x))) (o x y)))
+             ∃# (fun x : b => (∃# (fun x0 : a => m' x0 ∧# n x0 x)) ∧# o x y))
           (fun y : c =>
-             existsHash (fun x : a =>
-                           andHash (m' x)
-                             (existsHash (fun x0 : b =>
-                                            andHash (n x x0) (o x0 y)))))).
+             ∃# (fun x : a => m' x ∧# (∃# (fun x0 : b => n x x0 ∧# o x0 y))))).
   assert (forall x : c,
-             existsHash (fun x0 : b =>
-                           andHash (existsHash (fun x1 : a =>
-                                                  andHash (m' x1)
-                                                    (n x1 x0))) (o x0 x)) =
-               existsHash (fun x0 : a =>
-                             andHash (m' x0)
-                               (existsHash (fun x1 : b =>
-                                              andHash (n x0 x1)
-                                                (o x1 x))))).
+             (∃# (fun x0 : b =>
+                   (∃# (fun x1 : a => m' x1 ∧# n x1 x0)) ∧# (o x0 x))) =
+               ∃# (fun x0 : a =>
+                     m' x0 ∧# (∃# (fun x1 : b => n x0 x1 ∧# o x1 x)))).
   intro.
   exact (existsHash_andHash_existsHash_andHash
            m' (fun x y => n y x) (fun x1 => o x1 x)).
